git/cruhland/lean4-axiomatic/Lean4Axiomatic/Integer/Core.lean
@@ -8,31 +8,84 @@ import Lean4Axiomatic.Relation.Equivalence
 namespace Lean4Axiomatic.Integer
 
 /--
-Definitions pertaining to equality of integer values.
+Definitions pertaining to equivalence of integer values.
 
 **Named parameters**
-- `ℤ`: The type of integers.
+- `ℤ`: The integers.
 -/
-class Equality (ℤ : Type) :=
-  /-- The equality relation on integers, expressed with the syntax `a ≃ b`. -/
+class Equivalence (ℤ : Type) :=
+  /--
+  The standard equivalence relation on integers, expressed with the syntax
+  `a ≃ b`.
+  -/
   eqvOp : Relation.Equivalence.EqvOp ℤ
 
-attribute [instance] Equality.eqvOp
+attribute [instance] Equivalence.eqvOp
 
 /--
 Definitions pertaining to conversion of other types into or out of integers.
 
 **Named parameters**
-- `ℕ`: A type that implements the natural numbers.
-- `ℤ`: The type of integers.
+- `ℕ`: The natural numbers.
+- `ℤ`: The integers.
+
+**Class parameters**
+- `Natural ℕ`: Evidence that `ℕ` implements the natural numbers.
+- All other class parameters provide the subset of integer properties necessary
+  to define the fields of this class.
+-/
+class Conversion
+    (ℕ : outParam Type) [outParam (Natural ℕ)]
+    (ℤ : outParam Type) [outParam (Equivalence ℤ)]
+    :=
+  /-- Every natural number has an integer representation. -/
+  from_natural : Coe ℕ ℤ
+
+  /-- Every natural number maps to a unique integer. -/
+  from_natural_substitutive
+    : AA.Substitutive₁ (α := ℕ) (β := ℤ) (↑·) (· ≃ ·) (· ≃ ·)
+
+  /-- Every integer representation comes from a unique natural number. -/
+  from_natural_injective : AA.Injective (α := ℕ) (β := ℤ) (↑·) (· ≃ ·) (· ≃ ·)
+
+attribute [instance] Conversion.from_natural
+attribute [instance] Conversion.from_natural_injective
+attribute [instance] Conversion.from_natural_substitutive
+
+/--
+Bundles all core integer classes into one, to reduce the number of core
+dependencies needed by other integer classes.
+
+**Named parameters**
+- `ℕ`: The natural numbers.
+- `ℤ`: The integers.
 
 **Class parameters**
 - `Natural ℕ`: Evidence that `ℕ` implements the natural numbers.
 -/
-class Conversion (ℕ : Type) [Natural ℕ] (ℤ : Type) :=
-  /-- Every natural number has an integer representation. -/
-  from_natural : Coe ℕ ℤ
+class Core.Base (ℕ : outParam Type) [outParam (Natural ℕ)] (ℤ : outParam Type)
+  extends Equivalence ℤ, Conversion ℕ ℤ
 
-attribute [instance] Conversion.from_natural
+/--
+Properties that follow from those provided by `Core.Base`.
+
+**Named parameters**
+- `ℕ`: The natural numbers.
+- `ℤ`: The integers.
+
+**Class parameters**
+- `Natural ℕ`: Evidence that `ℕ` implements the natural numbers.
+-/
+class Core.Derived
+    (ℕ : outParam Type) [outParam (Natural ℕ)] (ℤ : outParam Type)
+    extends Core.Base ℕ ℤ
+    :=
+  /-- The integer values for zero and one are not equivalent. -/
+  one_neqv_zero : (1 : ℤ) ≄ 0
+
+namespace Core
+export Core.Derived (one_neqv_zero)
+export Equivalence (eqvOp)
+end Core
 
 end Lean4Axiomatic.Integer
