git/cruhland/lean4-axiomatic/Lean4Axiomatic/Integer/Impl/Derived/Negation.lean
@@ -5,11 +5,14 @@ namespace Lean4Axiomatic.Integer.Impl.Derived
 variable {ℕ : Type}
 variable [Natural ℕ]
 variable {ℤ : Type}
-variable [Equality ℤ]
-variable [Conversion ℕ ℤ]
+variable [Core.Derived ℕ ℤ]
 variable [Addition.Base ℕ ℤ]
 variable [Multiplication.Base ℕ ℤ]
 variable [Negation.Base ℕ ℤ]
+
+namespace Base
+export Negation (trichotomy)
+end Base
 
 /--
 Zero is a left absorbing element for multiplication.
@@ -79,16 +82,424 @@ def neg_semicompatibleL_mul
   scompat := neg_scompatL_mul
 }
 
-def neg_semicompatible_mul : AA.Semicompatible (α := ℤ) (-·) (· * ·) := {
+local instance neg_semicompatible_mul
+    : AA.Semicompatible (α := ℤ) (-·) (· * ·)
+    := {
   semicompatibleL :=
     neg_semicompatibleL_mul
   semicompatibleR :=
     AA.semicompatibleR_from_semicompatibleL neg_semicompatibleL_mul
 }
 
-def negation_derived : Negation.Derived ℕ ℤ := {
+/--
+Negation is an involution; applying it twice is equivalent to not applying it
+at all.
+
+**Property intuition**: Negation transforms an integer into its "mirror image"
+reflection across zero. Reflecting twice gives back the original integer.
+
+**Proof intuition**: The value `-a` is the additive inverse of `-(-a)` and also
+`a`. Thus, it can be used as an intermediate to replace one with the other.
+-/
+theorem neg_involutive {a : ℤ} : -(-a) ≃ a := calc
+  -(-a)            ≃ _ := Rel.symm AA.identL
+  0 + -(-a)        ≃ _ := AA.substL (Rel.symm AA.inverseR)
+  (a + -a) + -(-a) ≃ _ := AA.assoc
+  a + (-a + -(-a)) ≃ _ := AA.substR AA.inverseR
+  a + 0            ≃ _ := AA.identR
+  a                ≃ _ := Rel.refl
+
+/--
+A positive or negative integer of unit magnitude.
+
+Only `1` and `-1` satisfy this property. It's formulated using multiplication
+to be easy to use with algebra.
+
+**Named parameters**
+- `a`: The integer satisfying the property.
+-/
+def SquareRootOfUnity (a : ℤ) : Prop := a * a ≃ 1
+
+/--
+A positive or negative integer.
+
+Represents nonzero integers as the product of a nonzero sign (`1` or `-1`) and
+a positive magnitude. This is convenient for use in algebraic proofs.
+
+**Named parameters**
+- `a`: The integer satisfying the property.
+-/
+inductive Nonzero (a : ℤ) : Prop :=
+| /--
+  Construct evidence that the integer `a` is nonzero.
+
+  **Named parameters**
+  - `sign`: Has value `1` if `a` is positive, or `-1` if `a` is negative.
+  - `magnitude`: The distance of `a` from zero, as a natural number.
+  - `sqrt_1`: Evidence that `sign` is `1` or `-1`.
+  - `pos`: Evidence that `magnitude` is positive.
+  - `prod`: Evidence that `a` is a positive or negative value.
+  -/
+  intro
+    (sign : ℤ)
+    (magnitude : ℕ)
+    (sqrt_1 : SquareRootOfUnity sign)
+    (pos : Natural.Positive magnitude)
+    (prod : a ≃ sign * ↑magnitude)
+
+/--
+Expresses that one of two propositions is true, but not both.
+
+**Named parameters**
+- `α`, `β`: The two propositions.
+-/
+def ExactlyOneOfTwo (α β : Prop) : Prop := (α ∨ β) ∧ ¬ (α ∧ β)
+
+section
+
+open Natural (step)
+
+/--
+Zero is the only natural number less than one.
+
+This is a lemma to help with the proof of `natural_sqrt_1` below.
+-/
+theorem zero_lt_one {n : ℕ} : n < 1 ↔ n ≃ 0 := by
+  apply Iff.intro
+  case mp =>
+    intro (_ : n < 1)
+    show n ≃ 0
+    have : n < step 0 := AA.substRFn Natural.literal_step ‹n < 1›
+    have : n < 0 ∨ n ≃ 0 := Natural.lt_split ‹n < step 0›
+    match ‹n < 0 ∨ n ≃ 0› with
+    | Or.inl (_ : n < 0) => exact absurd ‹n < 0› Natural.lt_zero
+    | Or.inr (_ : n ≃ 0) => exact ‹n ≃ 0›
+  case mpr =>
+    intro (_ : n ≃ 0)
+    show n < 1
+    have : (0 : ℕ) < step 0 := Natural.lt_step
+    have : n < step 0 := AA.substLFn (Rel.symm ‹n ≃ 0›) ‹(0 : ℕ) < step 0›
+    have : n < 1 := AA.substRFn (Rel.symm Natural.literal_step) ‹n < step 0›
+    exact ‹n < 1›
+
+/--
+The only square root of unity in the natural numbers is `1`.
+
+**Property and proof intuition**: It can only be one, because zero squared is
+zero, and squaring any natural number greater than one always produces a larger
+result.
+-/
+theorem natural_sqrt_1 {n : ℕ} : n * n ≃ 1 ↔ n ≃ 1 := by
+  apply Iff.intro
+  case mp =>
+    intro (_ : n * n ≃ 1)
+    show n ≃ 1
+    have tri_n_1 : AA.ExactlyOneOfThree (n < 1) (n ≃ 1) (n > 1) :=
+      Natural.trichotomy n 1
+    match tri_n_1.atLeastOne with
+    | AA.OneOfThree.first (_ : n < 1) =>
+      apply False.elim
+      show False
+      have : n ≃ 0 := zero_lt_one.mp ‹n < 1›
+      have : step 0 ≃ 0 := calc
+        step 0  ≃ _ := Rel.symm Natural.literal_step
+        1       ≃ _ := Rel.symm ‹n * n ≃ 1›
+        n * n   ≃ _ := AA.substL ‹n ≃ 0›
+        0 * n   ≃ _ := AA.absorbL
+        0       ≃ _ := Rel.refl
+      exact absurd ‹step (0 : ℕ) ≃ 0› Natural.step_neq_zero
+    | AA.OneOfThree.second (_ : n ≃ 1) =>
+      exact ‹n ≃ 1›
+    | AA.OneOfThree.third (_ : n > 1) =>
+      apply False.elim
+      show False
+      apply tri_n_1.atMostOne
+      show AA.TwoOfThree (n < 1) (n ≃ 1) (n > 1)
+      have : step 0 < n := AA.substLFn Natural.literal_step ‹1 < n›
+      have : 0 < n := Rel.trans Natural.lt_step ‹step 0 < n›
+      have : Natural.Positive n := Natural.lt_zero_pos.mpr ‹0 < n›
+      have : 1 * n < n * n := AA.substLC ‹Natural.Positive n› ‹1 < n›
+      have : n < n * n := AA.substLFn AA.identL ‹1 * n < n * n›
+      have : n < 1 := AA.substRFn ‹n * n ≃ 1› ‹n < n * n›
+      exact AA.TwoOfThree.oneAndThree ‹n < 1› ‹n > 1›
+  case mpr =>
+    intro (_ : n ≃ 1)
+    show n * n ≃ 1
+    calc
+      n * n ≃ _ := AA.substL ‹n ≃ 1›
+      1 * n ≃ _ := AA.identL
+      n     ≃ _ := ‹n ≃ 1›
+      1     ≃ _ := Rel.refl
+
+end
+
+/--
+The only square roots of unity in the integers are `1` and `-1`.
+
+**Property and proof intuition**: This follows from similar reasoning as
+`natural_sqrt_1`. Zero squared is zero, and integers greater than one or less
+than negative one all have squares that are greater than one.
+-/
+theorem sqrt_1_cases {a : ℤ} : SquareRootOfUnity a ↔ a ≃ 1 ∨ a ≃ -1 := by
+  apply Iff.intro
+  case mp =>
+    intro (_ : a * a ≃ 1)
+    show a ≃ 1 ∨ a ≃ -1
+    have from_nat_subst :=
+      @AA.subst₁ (self := Conversion.from_natural_substitutive)
+    match (Base.trichotomy a).atLeastOne with
+    | AA.OneOfThree.first
+        (_ : a ≃ 0) =>
+      apply False.elim
+      show False
+      have : 1 ≃ 0 := calc
+        1       ≃ _ := Rel.symm ‹a * a ≃ 1›
+        a * a   ≃ _ := AA.substL ‹a ≃ 0›
+        0 * a   ≃ _ := AA.absorbL
+        0       ≃ _ := Rel.refl
+      exact absurd ‹(1 : ℤ) ≃ 0› Core.one_neqv_zero
+    | AA.OneOfThree.second
+        (Exists.intro n (And.intro (_ : Natural.Positive n) (_ : a ≃ ↑n))) =>
+      apply Or.inl
+      show a ≃ 1
+      have : ↑(n * n) ≃ ↑(1 : ℕ) := calc
+        ↑(n * n) ≃ _ := AA.compat₂ (f := (↑·))
+        ↑n * ↑n  ≃ _ := AA.substL (Rel.symm ‹a ≃ ↑n›)
+        a * ↑n   ≃ _ := AA.substR (Rel.symm ‹a ≃ ↑n›)
+        a * a    ≃ _ := ‹a * a ≃ 1›
+        1        ≃ _ := Rel.refl
+      have : n * n ≃ 1 := AA.inject ‹↑(n * n) ≃ ↑(1 : ℕ)›
+      have : n ≃ 1 := natural_sqrt_1.mp ‹n * n ≃ 1›
+      calc
+        a       ≃ _ := ‹a ≃ ↑n›
+        ↑n      ≃ _ := from_nat_subst ‹n ≃ 1›
+        ↑1      ≃ _ := Rel.refl
+        (1 : ℤ) ≃ _ := Rel.refl
+    | AA.OneOfThree.third
+        (Exists.intro n (And.intro (_ : Natural.Positive n) (_ : a ≃ -↑n))) =>
+      apply Or.inr
+      show a ≃ -1
+      have : ↑(n * n) ≃ ↑(1 : ℕ) := calc
+        ↑(n * n)        ≃ _ := AA.compat₂ (f := (↑·))
+        ↑n * ↑n         ≃ _ := Rel.symm neg_involutive
+        (-(-(↑n * ↑n))) ≃ _ := AA.subst₁ AA.scompatR
+        (-(↑n * -↑n))   ≃ _ := AA.scompatL
+        (-↑n) * (-↑n)   ≃ _ := AA.substL (Rel.symm ‹a ≃ -↑n›)
+        a * (-↑n)       ≃ _ := AA.substR (Rel.symm ‹a ≃ -↑n›)
+        a * a           ≃ _ := ‹a * a ≃ 1›
+        1               ≃ _ := Rel.refl
+      have : n * n ≃ 1 := AA.inject ‹↑(n * n) ≃ ↑(1 : ℕ)›
+      have : n ≃ 1 := natural_sqrt_1.mp ‹n * n ≃ 1›
+      calc
+        a     ≃ _ := ‹a ≃ -↑n›
+        (-↑n) ≃ _ := AA.subst₁ (from_nat_subst ‹n ≃ 1›)
+        (-↑1) ≃ _ := Rel.refl
+        (-1)  ≃ _ := Rel.refl
+  case mpr =>
+    intro (_ : a ≃ 1 ∨ a ≃ -1)
+    show a * a ≃ 1
+    match ‹a ≃ 1 ∨ a ≃ -1› with
+    | Or.inl (_ : a ≃ 1) => calc
+      a * a ≃ _ := AA.substL ‹a ≃ 1›
+      1 * a ≃ _ := AA.identL
+      a     ≃ _ := ‹a ≃ 1›
+      1     ≃ _ := Rel.refl
+    | Or.inr (_ : a ≃ -1) => calc
+      a * a      ≃ _ := AA.substR ‹a ≃ -1›
+      a * -1     ≃ _ := Rel.symm AA.scompatR
+      (-(a * 1)) ≃ _ := AA.subst₁ AA.identR
+      (-a)       ≃ _ := AA.subst₁ ‹a ≃ -1›
+      (-(-1))    ≃ _ := neg_involutive
+      1          ≃ _ := Rel.refl
+
+/--
+Provide evidence that an integer is equivalent, or not equivalent, to zero.
+
+**Property and proof intuition**: We already know from trichotomy of integers
+that every integer is either zero, positive, or negative, and never more than
+one of those at the same time. Combine the positive and negative categories to
+obtain this result.
+-/
+theorem zero? (a : ℤ) : ExactlyOneOfTwo (a ≃ 0) (Nonzero a) := by
+  have tri : AA.ExactlyOneOfThree
+      (a ≃ 0)
+      (∃ n, Natural.Positive n ∧ a ≃ ↑n)
+      (∃ n, Natural.Positive n ∧ a ≃ -↑n)
+      :=
+    Base.trichotomy a
+  apply And.intro
+  case left =>
+    show a ≃ 0 ∨ Nonzero a
+    match tri.atLeastOne with
+    | AA.OneOfThree.first (_ : a ≃ 0) =>
+      exact Or.inl ‹a ≃ 0›
+    | AA.OneOfThree.second (a_pos : ∃ n, Natural.Positive n ∧ a ≃ ↑n) =>
+      have (Exists.intro n (And.intro (_ : Natural.Positive n) (_ : a ≃ ↑n)))
+        := a_pos
+      apply Or.inr
+      show Nonzero a
+      apply Nonzero.intro 1 n
+      case h.sqrt_1 =>
+        show SquareRootOfUnity 1
+        exact sqrt_1_cases.mpr (Or.inl Rel.refl)
+      case h.pos =>
+        show Natural.Positive n
+        exact ‹Natural.Positive n›
+      case h.prod =>
+        show a ≃ 1 * ↑n
+        calc
+          a      ≃ _ := ‹a ≃ ↑n›
+          ↑n     ≃ _ := Rel.symm AA.identL
+          1 * ↑n ≃ _ := Rel.refl
+    | AA.OneOfThree.third (a_neg : ∃ n, Natural.Positive n ∧ a ≃ -↑n) =>
+      have (Exists.intro n (And.intro (_ : Natural.Positive n) (_ : a ≃ -↑n)))
+        := a_neg
+      apply Or.inr
+      show Nonzero a
+      apply Nonzero.intro (-1) n
+      case h.sqrt_1 =>
+        show SquareRootOfUnity (-1)
+        exact sqrt_1_cases.mpr (Or.inr Rel.refl)
+      case h.pos =>
+        show Natural.Positive n
+        exact ‹Natural.Positive n›
+      case h.prod =>
+        show a ≃ -1 * ↑n
+        calc
+          a           ≃ _ := ‹a ≃ -↑n›
+          (-↑n)       ≃ _ := AA.subst₁ (Rel.symm AA.identL)
+          (-(1 * ↑n)) ≃ _ := AA.scompatL
+          (-1) * ↑n   ≃ _ := Rel.refl
+  case right =>
+    intro (And.intro (_ : a ≃ 0) (_ : Nonzero a))
+    show False
+    apply tri.atMostOne
+    show AA.TwoOfThree
+      (a ≃ 0)
+      (∃ n, Natural.Positive n ∧ a ≃ ↑n)
+      (∃ n, Natural.Positive n ∧ a ≃ -↑n)
+    have (Nonzero.intro s m
+        (_ : SquareRootOfUnity s) (_ : Natural.Positive m) (_ : a ≃ s * ↑m))
+      := ‹Nonzero a›
+    have : s ≃ 1 ∨ s ≃ -1 := sqrt_1_cases.mp ‹SquareRootOfUnity s›
+    match ‹s ≃ 1 ∨ s ≃ -1› with
+    | Or.inl (_ : s ≃ 1) =>
+      have : a ≃ ↑m := calc
+        a      ≃ _ := ‹a ≃ s * ↑m›
+        s * ↑m ≃ _ := AA.substL ‹s ≃ 1›
+        1 * ↑m ≃ _ := AA.identL
+        ↑m     ≃ _ := Rel.refl
+      have : ∃ n, Natural.Positive n ∧ a ≃ ↑n :=
+        Exists.intro m (And.intro ‹Natural.Positive m› ‹a ≃ ↑m›)
+      exact AA.TwoOfThree.oneAndTwo ‹a ≃ 0› ‹∃ n, Natural.Positive n ∧ a ≃ ↑n›
+    | Or.inr (_ : s ≃ -1) =>
+      have : a ≃ -↑m := calc
+        a           ≃ _ := ‹a ≃ s * ↑m›
+        s * ↑m      ≃ _ := AA.substL ‹s ≃ -1›
+        (-1) * ↑m   ≃ _ := Rel.symm AA.scompatL
+        (-(1 * ↑m)) ≃ _ := AA.subst₁ AA.identL
+        (-↑m)       ≃ _ := Rel.refl
+      have : ∃ n, Natural.Positive n ∧ a ≃ -↑n :=
+        Exists.intro m (And.intro ‹Natural.Positive m› ‹a ≃ -↑m›)
+      exact
+        AA.TwoOfThree.oneAndThree ‹a ≃ 0› ‹∃ n, Natural.Positive n ∧ a ≃ -↑n›
+
+/--
+The product of nonzero integers is nonzero.
+
+**Property and proof intuition**: Integers can be viewed as natural numbers
+(i.e. magnitudes) with signs (i.e. one-dimensional directions). We already
+know that nonzero natural numbers are preserved under multiplication. The same
+is true for signs: the sign of a product will never be zero if the factors also
+have nonzero (i.e. positive or negative) signs. Thus there is no way for a
+product of nonzero integers to become zero.
+-/
+theorem mul_preserves_nonzero
+    {a b : ℤ} : Nonzero a → Nonzero b → Nonzero (a * b)
+    := by
+  intro (Nonzero.intro as am
+      (_ : SquareRootOfUnity as) (_ : Natural.Positive am) (_ : a ≃ as * ↑am))
+  intro (Nonzero.intro bs bm
+      (_ : SquareRootOfUnity bs) (_ : Natural.Positive bm) (_ : b ≃ bs * ↑bm))
+  show Nonzero (a * b)
+  apply Nonzero.intro (as * bs) (am * bm)
+  case sqrt_1 =>
+    show SquareRootOfUnity (as * bs)
+    have : as * as ≃ 1 := ‹SquareRootOfUnity as›
+    have : bs * bs ≃ 1 := ‹SquareRootOfUnity bs›
+    show (as * bs) * (as * bs) ≃ 1
+    calc
+      (as * bs) * (as * bs) ≃ _ := AA.expr_xxfxxff_lr_swap_rl
+      (as * as) * (bs * bs) ≃ _ := AA.substL ‹as * as ≃ 1›
+      1 * (bs * bs)         ≃ _ := AA.substR ‹bs * bs ≃ 1›
+      1 * 1                 ≃ _ := AA.identL
+      1                     ≃ _ := Rel.refl
+  case pos =>
+    show Natural.Positive (am * bm)
+    exact Natural.mul_positive ‹Natural.Positive am› ‹Natural.Positive bm›
+  case prod =>
+    show a * b ≃ (as * bs) * ↑(am * bm)
+    calc
+      a * b
+        ≃ _ := AA.substL ‹a ≃ as * ↑am›
+      (as * ↑am) * b
+        ≃ _ := AA.substR ‹b ≃ bs * ↑bm›
+      (as * ↑am) * (bs * ↑bm)
+        ≃ _ := AA.expr_xxfxxff_lr_swap_rl
+      (as * bs) * (↑am * ↑bm)
+        ≃ _ := AA.substR (Rel.symm (AA.compat₂ (f := (↑·))))
+      (as * bs) * ↑(am * bm)
+        ≃ _ := Rel.refl
+
+/--
+For a product of integers to be zero, at least one of its factors must be zero.
+
+**Property and proof intuition**: This property alone is not very intuitive, or
+at least the forward direction isn't. But eliminating the obvious cases where
+either `a` or `b` are zero reduces the problem to showing that if `a` and `b`
+are both nonzero, then their product must be nonzero as well. And that has some
+intuitive justification; see `mul_preserves_nonzero`.
+-/
+theorem mul_split_zero {a b : ℤ} : a * b ≃ 0 ↔ a ≃ 0 ∨ b ≃ 0 := by
+  apply Iff.intro
+  case mp =>
+    intro (_ : a * b ≃ 0)
+    show a ≃ 0 ∨ b ≃ 0
+    have : a ≃ 0 ∨ Nonzero a := (zero? a).left
+    match ‹a ≃ 0 ∨ Nonzero a› with
+    | Or.inl (_ : a ≃ 0) =>
+      exact Or.inl ‹a ≃ 0›
+    | Or.inr (_ : Nonzero a) =>
+      have : b ≃ 0 ∨ Nonzero b := (zero? b).left
+      match ‹b ≃ 0 ∨ Nonzero b› with
+      | Or.inl (_ : b ≃ 0) =>
+        exact Or.inr ‹b ≃ 0›
+      | Or.inr (_ : Nonzero b) =>
+        apply False.elim
+        show False
+        have : ¬ (a * b ≃ 0 ∧ Nonzero (a * b)) := (zero? (a * b)).right
+        apply this
+        show a * b ≃ 0 ∧ Nonzero (a * b)
+        apply And.intro
+        · exact ‹a * b ≃ 0›
+        · exact mul_preserves_nonzero ‹Nonzero a› ‹Nonzero b›
+  case mpr =>
+    intro (_ : a ≃ 0 ∨ b ≃ 0)
+    show a * b ≃ 0
+    match ‹a ≃ 0 ∨ b ≃ 0› with
+    | Or.inl (_ : a ≃ 0) => calc
+      a * b ≃ _ := AA.substL ‹a ≃ 0›
+      0 * b ≃ _ := AA.absorbL
+      0     ≃ _ := Rel.refl
+    | Or.inr (_ : b ≃ 0) => calc
+      a * b ≃ _ := AA.substR ‹b ≃ 0›
+      a * 0 ≃ _ := AA.absorbR
+      0     ≃ _ := Rel.refl
+
+def negation : Negation.Derived ℕ ℤ := {
   mul_absorbing := mul_absorbing
   neg_semicompatible_mul := neg_semicompatible_mul
+  neg_involutive := neg_involutive
 }
 
 end Lean4Axiomatic.Integer.Impl.Derived
