git/cruhland/lean4-axiomatic/Lean4Axiomatic/Integer/Multiplication.lean
@@ -13,14 +13,17 @@ Definition of multiplication, and properties that it must satisfy.
 All other properties of multiplication can be derived from these.
 
 **Named parameters**
-- `ℤ`: The type of integers.
+- `ℕ`: The natural numbers.
+- `ℤ`: The integers.
 
 **Class parameters**
-- `Equality ℤ`: Required to express most properties of multiplication.
+- `Natural ℕ`: Evidence that `ℕ` implements the natural numbers.
+- All other class parameters provide the subset of integer properties necessary
+  to define the fields of this class.
 -/
 class Multiplication.Base
-    (ℕ : Type) [Natural ℕ]
-    (ℤ : Type) [Equality ℤ] [Conversion ℕ ℤ] [Addition.Base ℕ ℤ]
+    (ℕ : outParam Type) [outParam (Natural ℕ)]
+    (ℤ : Type) [outParam (Core.Base ℕ ℤ)] [outParam (Addition.Base ℕ ℤ)]
     :=
   /-- Definition of and syntax for multiplication. -/
   mulOp : Mul ℤ
@@ -46,9 +49,19 @@ class Multiplication.Base
   -/
   mul_distributive : AA.Distributive (α := ℤ) (· * ·) (· + ·)
 
+  /--
+  Multiplying two natural numbers and then converting to an integer gives the
+  same result as converting each number to an integer and then multiplying.
+  -/
+  mul_compatible_from_natural
+    : AA.Compatible₂ (α := ℕ) (β := ℤ) (↑·) (· * ·) (· * ·)
+
 attribute [instance] Multiplication.Base.mulOp
+attribute [instance] Multiplication.Base.mul_associative
 attribute [instance] Multiplication.Base.mul_commutative
+attribute [instance] Multiplication.Base.mul_compatible_from_natural
 attribute [instance] Multiplication.Base.mul_distributive
+attribute [instance] Multiplication.Base.mul_identity
 attribute [instance] Multiplication.Base.mul_substitutive
 
 namespace Multiplication
