git/cruhland/lean4-axiomatic/Lean4Axiomatic/Integer/Negation.lean
@@ -14,14 +14,17 @@ Definition of negation, and properties that it must satisfy.
 All other properties of negation can be derived from these.
 
 **Named parameters**
-- `ℤ`: The type of integers.
+- `ℕ`: The natural numbers.
+- `ℤ`: The integers.
 
 **Class parameters**
-- `Equality ℤ`: Required to express most properties of negation.
+- `Natural ℕ`: Evidence that `ℕ` implements the natural numbers.
+- All other class parameters provide the subset of integer properties necessary
+  to define the fields of this class.
 -/
 class Negation.Base
-    (ℕ : Type) [Natural ℕ]
-    (ℤ : Type) [Equality ℤ] [Conversion ℕ ℤ] [Addition.Base ℕ ℤ]
+    (ℕ : outParam Type) [outParam (Natural ℕ)]
+    (ℤ : Type) [outParam (Core.Base ℕ ℤ)] [outParam (Addition.Base ℕ ℤ)]
     :=
   /-- Definition of and syntax for negation. -/
   negOp : Neg ℤ
@@ -33,7 +36,7 @@ class Negation.Base
   neg_substitutive : AA.Substitutive₁ (α := ℤ) (-·) (· ≃ ·) (· ≃ ·)
 
   /-- Every integer is either positive, negative, or zero. -/
-  trichotomy {a : ℤ}
+  trichotomy (a : ℤ)
     : AA.ExactlyOneOfThree
       (a ≃ ↑(0 : ℕ))
       (∃ (n : ℕ), Natural.Positive n ∧ a ≃ n)
@@ -46,20 +49,34 @@ attribute [instance] Negation.Base.negOp
 attribute [instance] Negation.Base.neg_inverse
 attribute [instance] Negation.Base.neg_substitutive
 
-/-- Properties that follow from those provided in `Negation.Base`. -/
+/--
+Properties that follow from those provided in `Negation.Base`.
+
+**Named parameters**
+- `ℕ`: The natural numbers.
+- `ℤ`: The integers.
+
+**Class parameters**
+- `Natural ℕ`: Evidence that `ℕ` implements the natural numbers.
+- All other class parameters provide the subset of integer properties necessary
+  to define the fields of this class.
+-/
 class Negation.Derived
     (ℕ : Type) [Natural ℕ]
-    (ℤ : Type) [Equality ℤ] [Conversion ℕ ℤ]
-    [Addition.Base ℕ ℤ] [Multiplication.Base ℕ ℤ]
-    extends Negation.Base ℕ ℤ :=
+    (ℤ : Type) [Core.Base ℕ ℤ] [Addition.Base ℕ ℤ] [Multiplication.Base ℕ ℤ]
+    extends Negation.Base ℕ ℤ
+    :=
   /-- Multiplying by zero always gives zero. -/
   mul_absorbing : AA.Absorbing (α := ℤ) 0 (· * ·)
 
   /-- Negation can be moved between a product and either one of its factors. -/
   neg_semicompatible_mul : AA.Semicompatible (α := ℤ) (-·) (· * ·)
 
+  /-- Negation cancels out negation. -/
+  neg_involutive {a : ℤ} : -(-a) ≃ a
+
 namespace Negation
-export Negation.Base (negOp)
+export Negation.Base (negOp trichotomy)
 end Negation
 
 end Lean4Axiomatic.Integer
