git/cruhland/lean4-axiomatic/Lean4Axiomatic/Integer/Subtraction.lean
@@ -13,12 +13,13 @@ Definition of subtraction, and properties that it must satisfy.
 All other properties of subtraction can be derived from these.
 
 **Named parameters**
-- `ℤ`: The type of integers.
+- `ℤ`: The integers.
 
 **Class parameters**
-- `Equality ℤ`: Needed to express some properties of subtraction.
+- All other class parameters provide the subset of integer properties necessary
+  to define the fields of this class.
 -/
-class Subtraction.Base (ℤ : Type) [Equality ℤ] :=
+class Subtraction.Base (ℤ : Type) [Equivalence ℤ] :=
   /-- Definition of and syntax for subtraction. -/
   subOp : Sub ℤ
 
