git/cruhland/lean4-axiomatic/Lean4Axiomatic/Integer/Impl/Derived/Core.lean
@@ -1,0 +1,34 @@
+import Lean4Axiomatic.Integer.Core
+
+namespace Lean4Axiomatic.Integer.Impl.Derived
+
+/-! # Integer properties derived from `Core.Base` -/
+
+variable {ℕ : Type}
+variable [Natural ℕ]
+variable {ℤ : Type}
+variable [Core.Base ℕ ℤ]
+
+/--
+The integer one is not the same as the integer zero.
+
+**Proof intuition**: All the laws of algebra for integers continue to hold if
+`0 ≃ 1` (see [zero ring](https://en.wikipedia.org/wiki/Zero_ring)), so we need
+to use a non-algebraic fact. This is provided by the mapping from natural
+numbers to integers, specifically its injectivity which allows us to translate
+the property that a successor is never the same as zero into the integers.
+-/
+theorem one_neqv_zero : (1 : ℤ) ≄ 0 := by
+  intro (_ : (1 : ℤ) ≃ 0)
+  show False
+  have : ↑(1 : ℕ) ≃ ↑(0 : ℕ) := ‹(1 : ℤ) ≃ 0›
+  have : (1 : ℕ) ≃ 0 := AA.inject ‹↑(1 : ℕ) ≃ ↑(0 : ℕ)›
+  have : Natural.step (0 : ℕ) ≃ 0 :=
+    Rel.trans (Rel.symm Natural.literal_step) ‹(1 : ℕ) ≃ 0›
+  exact absurd ‹Natural.step (0 : ℕ) ≃ 0› Natural.step_neq_zero
+
+instance core : Core.Derived ℕ ℤ := {
+  one_neqv_zero := one_neqv_zero
+}
+
+end Lean4Axiomatic.Integer.Impl.Derived
